Added rem-wins map + disable-wins flag

table.py
@@ -2,7 +2,6 @@ import subprocess
 import time
 from tabulate import tabulate
 
-# Function to execute command and measure time
 def execute_command(command):
     start_time = time.time()
     try:
@@ -15,8 +14,12 @@ def execute_command(command):
     elapsed_time = end_time - start_time
     return elapsed_time
 
-# List of commands to execute
 commands = [
+	#"fstar.exe interface/App_new.fsti",
+	"#fstar.exe interface/Set_extended.fsti",
+	"#fstar.exe interface/Set_extended.fst",
+	#"fstar.exe interface/Map_extended.fsti interface/Set_extended.fsti",
+	#"fstar.exe interface/Map_extended.fst interface/Set_extended.fsti",
 	"fstar.exe mrdts-new/Increment-only_counter/App_new.fst interface/App_new.fsti",
 	"fstar.exe mrdts-new/PN_counter/App_new.fst interface/App_new.fsti",
 	"fstar.exe mrdts-new/Grow-only_set/App_new.fst interface/App_new.fsti interface/Set_extended.fsti",
@@ -27,7 +30,6 @@ commands = [
 	"fstar.exe mrdts-new/Observed-remove_set_eff_new/App_new_new.fst interface/Set_extended.fsti interface/Map_extended.fsti",
 ]
 
-# Execute commands and measure execution time
 results = []
 total_execution_time = 0
 for command in commands:
@@ -36,7 +38,6 @@ for command in commands:
         total_execution_time += execution_time
         results.append([command, f"{execution_time:.4f} seconds"])
 
-# Print individual command execution times in tabular format
 if results:
     print(tabulate(results, headers=["Command", "Execution Time"]))
     print(f"\nOverall execution time: {total_execution_time:.4f} seconds")
