mrdts-new/Remove-wins_set/.#App_new.fst
@@ -1,0 +1,1 @@
+apple@apples-MacBook-Pro-2.local.66950
